src/3d/InlineSingletonRecords.fst
@@ -41,7 +41,11 @@ let simplify_atomic_field (env:env) (f:atomic_field)
   = let field = f.v in
     let field = 
       match field.field_type.v with
-      | Pointer _ -> failwith "Impossible: field types cannot be pointers"
+      | Pointer _ -> (
+        if Some? field.field_probe
+        then field
+        else failwith "Impossible: field types cannot be pointers"
+      ) 
       | Type_app hd _ args ->
         begin
         match H.try_find env hd.v with
